code/ecdsap256sha2/Hacl.Impl.ECDSA.fsti
@@ -30,7 +30,10 @@ open Hacl.Impl.ECDSA.MontgomeryMultiplication
 open Hacl.Impl.P256.Signature.Common
 
 open Hacl.Impl.P256.Compression
-open Hacl.Impl.ECDSA.P256SHA256.Signature
+
+open Hacl.Impl.ECDSA.P256SHA256.Signature.Agile
+open Hacl.Impl.ECDSA.P256SHA256.Signature.Blake2
+
 open Hacl.Impl.ECDSA.P256SHA256.Verification
 
 open Spec.P256.MontgomeryMultiplication
@@ -53,7 +56,7 @@ val ecdsa_p256_sha2_sign: result: lbuffer uint8 (size 64) -> mLen: size_t -> m: 
      (assert_norm (pow2 32 < pow2 61);
       let resultR = gsub result (size 0) (size 32) in 
       let resultS = gsub result (size 32) (size 32) in 
-      let r, s, flagSpec = Spec.ECDSA.ecdsa_signature SHA2_256 (uint_v mLen) (as_seq h0 m) (as_seq h0 privKey) (as_seq h0 k) in 
+      let r, s, flagSpec = Spec.ECDSA.ecdsa_signature_agile SHA2_256 (uint_v mLen) (as_seq h0 m) (as_seq h0 privKey) (as_seq h0 k) in 
       as_seq h1 resultR == nat_to_bytes_be 32 r /\
       as_seq h1 resultS == nat_to_bytes_be 32 s /\
       flag == flagSpec 
@@ -78,7 +81,7 @@ val ecdsa_p256_sha2_384_sign: result: lbuffer uint8 (size 64) -> mLen: size_t ->
      (assert_norm (pow2 32 < pow2 61);
       let resultR = gsub result (size 0) (size 32) in 
       let resultS = gsub result (size 32) (size 32) in 
-      let r, s, flagSpec = Spec.ECDSA.ecdsa_signature SHA2_384 (uint_v mLen) (as_seq h0 m) (as_seq h0 privKey) (as_seq h0 k) in 
+      let r, s, flagSpec = Spec.ECDSA.ecdsa_signature_agile SHA2_384 (uint_v mLen) (as_seq h0 m) (as_seq h0 privKey) (as_seq h0 k) in 
       as_seq h1 resultR == nat_to_bytes_be 32 r /\
       as_seq h1 resultS == nat_to_bytes_be 32 s /\
       flag == flagSpec 
@@ -103,12 +106,38 @@ val ecdsa_p256_sha2_512_sign: result: lbuffer uint8 (size 64) -> mLen: size_t ->
      (assert_norm (pow2 32 < pow2 61);
       let resultR = gsub result (size 0) (size 32) in 
       let resultS = gsub result (size 32) (size 32) in 
-      let r, s, flagSpec = Spec.ECDSA.ecdsa_signature SHA2_512 (uint_v mLen) (as_seq h0 m) (as_seq h0 privKey) (as_seq h0 k) in 
+      let r, s, flagSpec = Spec.ECDSA.ecdsa_signature_agile SHA2_512 (uint_v mLen) (as_seq h0 m) (as_seq h0 privKey) (as_seq h0 k) in 
       as_seq h1 resultR == nat_to_bytes_be 32 r /\
       as_seq h1 resultS == nat_to_bytes_be 32 s /\
       flag == flagSpec 
     )    
   )
+
+
+val ecdsa_signature_blake2: result: lbuffer uint8 (size 64) -> mLen: size_t -> m: lbuffer uint8 mLen ->
+  privKey: lbuffer uint8 (size 32) -> 
+  k: lbuffer uint8 (size 32) -> 
+  Stack uint64
+  (requires fun h -> 
+    live h result /\ live h m /\ live h privKey /\ live h k /\
+    disjoint result m /\
+    disjoint result privKey /\
+    disjoint result k /\
+    nat_from_bytes_be (as_seq h privKey) < prime_p256_order /\
+    nat_from_bytes_be (as_seq h k) < prime_p256_order
+  )
+  (ensures fun h0 flag h1 -> 
+    modifies (loc result) h0 h1 /\
+     (assert_norm (pow2 32 < pow2 61);
+      let resultR = gsub result (size 0) (size 32) in 
+      let resultS = gsub result (size 32) (size 32) in 
+      let r, s, flagSpec = Spec.ECDSA.ecdsa_signature_blake2 (uint_v mLen) (as_seq h0 m) (as_seq h0 privKey) (as_seq h0 k) in 
+      as_seq h1 resultR == nat_to_bytes_be 32 r /\
+      as_seq h1 resultS == nat_to_bytes_be 32 s /\
+      flag == flagSpec 
+    )    
+  )
+
 
 
 (* This code is not side channel resistant *)
